LocaleRefinement.thy
@@ -12,10 +12,12 @@ for
   lc :: "('cstate, 'event) LTS"
 + 
 fixes 
-  inv :: "'astate \<times> 'cstate \<Rightarrow> bool"
+  inv :: "'astate \<Rightarrow> 'cstate \<Rightarrow> bool"
+assumes
+  po_init: "\<forall>cs \<in> init lc. \<exists>as \<in> init la. inv as cs" and
+  po_step: "\<forall>as cs. inv as cs \<longrightarrow> (\<forall>ct \<in> trans lc. src ct = cs \<longrightarrow>
+                (\<exists>at \<in> trans la. src at = as \<and> lbl at = lbl ct \<and> inv (dst at) (dst ct)))"
 begin
-  definition sound :: bool where
-    "sound \<equiv> true"
 end
 
 
