LocaleSimulation.thy
@@ -18,14 +18,14 @@ for
 fixes
   r :: "('a \<times> 'c) set"
 assumes
-  rinit: "\<forall> cs \<in> init lc. \<exists> as \<in> init la. (as, cs) \<in> r" and
-  rtrans: "\<forall> as cs . (as, cs) \<in> r \<longrightarrow> (\<forall> ct \<in> trans lc. src ct = cs \<longrightarrow>
-              (\<exists> at \<in> trans la. src at = as \<and> lbl at = lbl ct \<and> (dst at, dst ct) \<in> r))"
+  rinit: "\<forall>cs \<in> init lc. \<exists>as \<in> init la. (as, cs) \<in> r" and
+  rtrans: "\<forall>as cs. (as, cs) \<in> r \<longrightarrow> (\<forall>ct \<in> trans lc. src ct = cs \<longrightarrow>
+              (\<exists>at \<in> trans la. src at = as \<and> lbl at = lbl ct \<and> (dst at, dst ct) \<in> r))"
 begin
 end
 
-text {* One simple property involving simulations is that the identity relation $Id$
-defines a simulation of an LTS $l$by itself. This is expressed and showed in a context
+text {* One simple property involving simulations is that the identity relation @{text "Id"}}
+defines a simulation of an LTS @{text l} by itself. This is expressed and showed in a context
 containing the definition of LTS, as follows: *}
 sublocale LTS \<subseteq>
           Simulation lts lts Id
@@ -42,14 +42,14 @@ end
 sublocale SimulationComposition \<subseteq> 
           Simulation la lc "r1 O r2"
 proof 
-  from sim1.rinit sim2.rinit show "\<forall> cs \<in> init lc. \<exists> as \<in> init la. (as, cs) \<in> r1 O r2"
-    unfolding relcomp_unfold by simp metis
+  from sim1.rinit sim2.rinit show "\<forall>cs \<in> init lc. \<exists>as \<in> init la. (as, cs) \<in> r1 O r2"
+    unfolding relcomp_unfold by fastforce
 next
   from sim1.rtrans sim2.rtrans 
   show "\<forall>as cs. (as, cs) \<in> r1 O r2 \<longrightarrow> 
-         (\<forall> ct \<in> trans lc. src ct = cs \<longrightarrow> 
-           (\<exists> at \<in> trans la. src at = as \<and> lbl at = lbl ct \<and> (dst at, dst ct) \<in> r1 O r2))"
-    unfolding relcomp_unfold by simp metis
+         (\<forall>ct \<in> trans lc. src ct = cs \<longrightarrow> 
+           (\<exists>at \<in> trans la. src at = as \<and> lbl at = lbl ct \<and> (dst at, dst ct) \<in> r1 O r2))"
+    unfolding relcomp_unfold by fastforce
 qed
 
 text {* We introduce the relation simulates on LTS. Is there a way to use the locale Simulation
@@ -61,14 +61,14 @@ for
   la :: "('a, 'ev) LTS" and lc :: "('c, 'ev) LTS"
 +
 assumes
-  "\<exists> r . ((\<forall> cs \<in> init lc. \<exists> as \<in> init la. (as, cs) \<in> r) \<and>
-          (\<forall> as cs . (as, cs) \<in> r \<longrightarrow> (\<forall> ct \<in> trans lc. src ct = cs \<longrightarrow>
-              (\<exists> at \<in> trans la. src at = as \<and> lbl at = lbl ct \<and> (dst at, dst ct) \<in> r))))"
+  rel: "\<exists>r. ((\<forall>cs \<in> init lc. \<exists>as \<in> init la. (as, cs) \<in> r) \<and>
+          (\<forall>as cs. (as, cs) \<in> r \<longrightarrow> (\<forall>ct \<in> trans lc. src ct = cs \<longrightarrow>
+              (\<exists>at \<in> trans la. src at = as \<and> lbl at = lbl ct \<and> (dst at, dst ct) \<in> r))))"
 begin
 end
 
 sublocale Simulation \<subseteq> Simulate la lc
-sorry
+  using rinit rtrans by unfold_locales auto
   
 sublocale LTS \<subseteq> Simulate l l
 by unfold_locales auto
@@ -82,6 +82,26 @@ begin
 end
 
 sublocale SimulateCompose \<subseteq> Simulate la lc
-sorry
+proof
+  from sim1.rel obtain rab where
+    rab: "\<forall>bs \<in> init lb. \<exists>as \<in> init la. (as, bs) \<in> rab"
+         "\<forall>as bs. (as, bs) \<in> rab \<longrightarrow> (\<forall>bt \<in> trans lb. src bt = bs \<longrightarrow>
+              (\<exists>at \<in> trans la. src at = as \<and> lbl at = lbl bt \<and> (dst at, dst bt) \<in> rab))"
+    by blast
+  from sim2.rel obtain rbc where
+    rbc: "\<forall>cs \<in> init lc. \<exists>bs \<in> init lb. (bs, cs) \<in> rbc"
+         "\<forall>bs cs. (bs, cs) \<in> rbc \<longrightarrow> (\<forall>ct \<in> trans lc. src ct = cs \<longrightarrow>
+              (\<exists>bt \<in> trans lb. src bt = bs \<and> lbl bt = lbl ct \<and> (dst bt, dst ct) \<in> rbc))"
+    by blast
+  from rab rbc show
+    "\<exists>r. (\<forall>cs\<in>init lc. \<exists>as\<in>init la. (as, cs) \<in> r) \<and>
+        (\<forall>as cs.
+            (as, cs) \<in> r \<longrightarrow>
+            (\<forall>ct\<in>trans lc.
+                src ct = cs \<longrightarrow>
+                (\<exists>at\<in>trans la.
+                    src at = as \<and> lbl at = lbl ct \<and> (dst at, dst ct) \<in> r)))"
+  by (intro exI[where x="rab O rbc"]) (fastforce simp: relcomp_unfold)
+qed
 
 end
